non-deterministic semantics

DensitySem.v
@@ -4,13 +4,26 @@ Require Export UnitarySem.
 
 Fixpoint c_eval (dim : nat) (c : com) : Superoperator (2^dim) (2^dim) :=
   match c with
-  | skip      => fun ρ => ρ (* We could change to (super I _), making the next lemma trivial *)
+  | skip      => super (I _) (*or: fun ρ => ρ  *)
   | seq c1 c2 => compose_super (c_eval dim c2) (c_eval dim c1)  
   | app u l   => super (ueval dim u l)
   | meas n    => Splus (super (@pad 2 n dim (∣0⟩⟨0∣))) (super (@pad 2 n dim (∣1⟩⟨1∣))) 
   | reset n   => Splus (super (@pad 2 n dim (∣0⟩⟨0∣))) (super (@pad 2 n dim (∣0⟩⟨1∣)))
   end.
 
+Lemma c_eval_ucom : forall (c : ucom) (dim : nat),
+    c_eval dim c = super (uc_eval dim c).
+Proof.
+  intros c dim.
+  induction c; trivial.
+  simpl. rewrite IHc1, IHc2.
+  unfold compose_super, super; simpl.
+  apply functional_extensionality. intros ρ.
+  Msimpl; repeat rewrite Mmult_assoc.
+  reflexivity.
+Qed.
+
+(* If skip is just id:
 Lemma c_eval_ucom : forall (c : ucom) (dim : nat) (ρ : Density (2^dim)),
     WF_Matrix _ _ ρ ->
     c_eval dim c ρ = super (uc_eval dim c) ρ.
@@ -25,8 +38,4 @@ Proof.
     easy.
   - simpl. reflexivity.
 Qed.
-
-(* Alternative lemma (requires change to skip):
-Lemma c_eval_ucom' : forall (c : ucom) (dim : nat),
-    c_eval dim c = super (uc_eval dim c).
 *)
