NDSem.v
@@ -1,0 +1,50 @@
+Require Import Quantum.
+Require Import List.
+Require Import SQIMP.
+Require Import UnitarySem.
+
+(* MOVE ELSEWHERE! *)
+Fixpoint enumerate_bool_lists (len : nat) : list (list bool) :=
+  match len with
+  | 0 => []
+  | S len' => map (cons true) (enumerate_bool_lists len') ++ map (cons false) (enumerate_bool_lists len')
+  end.
+
+Search (bool -> bool -> bool).
+
+(* Assumes f's domain is {t,f}^len *)
+(* Returns the arity of {x | f x = b} *)
+Definition count (len : nat) (f : list bool -> bool) (b : bool): nat :=
+  length (filter (fun l => (bool_eq (f l) b)) (enumerate_bool_lists len)).
+
+Search count.
+
+(* /MOVE *)
+
+(* But also move *)
+
+Definition norm {n} (ψ : Vector n) :=
+  sqrt (fst (ψ ∘ ψ†)).  
+
+Inductive nd_eval : forall dim, com -> Vector (2^dim) -> Vector (2^dim) -> Prop :=
+  | nd_app : forall dim n (u : Unitary n) (l : list nat) (ψ : Vector (2^dim)),
+      nd_eval dim (app u l) ψ ((ueval dim u l) × ψ)
+  | nd_meas0 : forall dim n (ψ : Vector (2^dim)),
+      let ψ' := @pad 2 n dim (∣0⟩⟨0∣) × ψ in 
+      nd_eval dim (meas n) ψ (scale (/(norm ψ')) ψ') 
+  | nd_meas1 : forall dim n (ψ : Vector (2^dim)),
+      let ψ' := @pad 2 n dim (∣1⟩⟨1∣) × ψ in
+      norm ψ' <> 0%R ->
+      nd_eval dim (meas n) ψ (scale (/(norm ψ')) ψ') 
+.
+
+
+
+Reserved Notation "dim '$' c '/' ψ '||' ψ'" (at level 80).
+
+Inductive nd_eval : forall dim, com -> Vector (2^dim) -> Vector (2^dim) -> Prop :=
+  | nd_app : forall dim n (u : Unitary n) (l : list nat) (ψ : Vector (2^dim)),
+    (dim $ app u l / ψ || ((ueval dim u l) × ψ))
+
+where "dim '$' c '/' ψ '||' ψ'" := (nd_eval dim c ψ ψ').
+                                                                              
